Add defs of EBBs and justified pais.

src/dafny/beacon/ForkChoiceHelpers.dfy
@@ -39,7 +39,7 @@ module ForkChoiceHelpers {
     // import opened SeqHelpers
    
     /**
-     *  The chain defined by a block.
+     *  The view defined by a block.
      *  
      *  @param  br      A hash root of a block.
      *  @param  store   A store (similar to the view of the validator).
@@ -64,20 +64,69 @@ module ForkChoiceHelpers {
     }
 
     /**
-     *  The strict prefix of a chain.
+     *  Same as above but using block roots and stores instead of blocks.
      */
-    function strictChain(br: Root, store: Store) : seq<BeaconBlock>
+    function chainRoots(br: Root, store: Store) : seq<Root>
         requires br in store.blocks.Keys
-        requires  store.blocks[br].slot > 0
         requires forall k :: k in store.blocks.Keys && store.blocks[k].slot > 0 ==>
             store.blocks[k].parent_root in store.blocks.Keys
             && store.blocks[store.blocks[k].parent_root].slot < store.blocks[k].slot 
 
+        ensures |chainRoots(br, store)| >= 1
+        /** All the root values collected must be in the store.blocks map. */
+        ensures forall r :: r in chainRoots(br, store) ==> r in store.blocks.Keys
+        /** The last root value id mapped to a block with slot 0. */
+        ensures store.blocks[chainRoots(br, store)[|chainRoots(br, store)| - 1]].slot == 0 
         //  Computation always terminates as slot number decreases (well-foundedness).
         decreases store.blocks[br].slot
     {
-        chain(store.blocks[br].parent_root, store)
+        if ( store.blocks[br].slot == 0 ) then
+            //  Should be the genesis block.
+            [ br ]
+        else 
+            [ br ] + chainRoots(store.blocks[br].parent_root, store)
     }
+
+     /**
+     *  The view defined by a block.
+     *  
+     *  @param  br      A hash root of a block.
+     *  @param  store   A store (similar to the view of the validator).
+     *  @returns        The ancestors of the block `br` in  `store`.
+     */
+    // function rootView(br: Root, store: Store) : seq<Root>
+    //     requires br in store.blocks.Keys
+    //     requires forall k :: k in store.blocks.Keys && store.blocks[k].slot > 0 ==>
+    //         store.blocks[k].parent_root in store.blocks.Keys
+    //         && store.blocks[store.blocks[k].parent_root].slot < store.blocks[k].slot 
+
+    //     ensures |view(br, store)| >= 1
+    //     ensures view(br, store)[|view(br, store)| - 1].slot == 0 
+    //     //  Computation always terminates as slot number decreases (well-foundedness).
+    //     decreases store.blocks[br].slot
+    // {
+    //     if ( store.blocks[br].slot == 0 ) then
+    //         //  Should be the genesis block.
+    //         [ br ]
+    //     else 
+    //         [ br ] + rootView(store.blocks[br].parent_root, store)
+    // }
+
+    /**
+     *  The strict prefix of a chain.
+     */
+    // function strictChain(br: Root, store: Store) : seq<BeaconBlock>
+    //     requires br in store.blocks.Keys
+    //     requires  store.blocks[br].slot > 0
+    //     requires forall k :: k in store.blocks.Keys && store.blocks[k].slot > 0 ==>
+    //         store.blocks[k].parent_root in store.blocks.Keys
+    //         && store.blocks[store.blocks[k].parent_root].slot < store.blocks[k].slot 
+
+    //     //  Computation always terminates as slot number decreases (well-foundedness).
+    //     decreases store.blocks[br].slot
+    // {
+    //     view(store.blocks[br].parent_root, store)
+    // }
 
 
     /**
@@ -130,10 +179,39 @@ module ForkChoiceHelpers {
     }
 
     /**
+     *  Same as above but using block roots and stores instead of blocks.
+     */
+    function computeFirstEBBIndexFromRoots(xb : seq<Root>, e :  Epoch, store: Store) : nat
+        requires |xb| >= 1
+        requires forall r :: r in xb ==> r in store.blocks.Keys 
+        /** Last block has slot 0. */
+        requires store.blocks[xb[|xb| - 1]].slot == 0 
+
+        /** The result is in the range of xb. */
+        ensures computeFirstEBBIndexFromRoots(xb, e, store) < |xb|
+        /** The slot of the result is bounded. */
+        ensures store.blocks[xb[computeFirstEBBIndexFromRoots(xb, e, store)]].slot as nat <= e as nat * SLOTS_PER_EPOCH as nat 
+        /** The prefix of xb[..result] has slots >  e * SLOTS_PER_EPOCH. */
+        ensures forall j :: 0 <= j < computeFirstEBBIndexFromRoots(xb, e, store) ==>
+            store.blocks[xb[j]].slot as nat > e as nat * SLOTS_PER_EPOCH as nat
+        decreases xb 
+    {
+        if |xb| == 1 then 
+            //  only one choice, must be the block with slot == 0
+            0
+        else if store.blocks[xb[0]].slot as nat <= e as nat * SLOTS_PER_EPOCH as nat then 
+            //  first block isd a good one
+            0
+        else 
+            //  first block has too large a slot, search suffix of xb.
+            1 + computeFirstEBBIndexFromRoots(xb[1..], e, store)
+    }
+
+    /**
      *  Compute the subsequence of indices of epoch boundary blocks.
      *  @param  xb  A sequence of blocks.
      *  @param  e   An epoch.
-     *  @returns    The sequence of EBBs indices in xb.
+     *  @returns    The sequence of EBBs indices in xb from epoch e to epoch 0.
      *  @note       We don't need the assumption that the list of blocks in `xb`
      *              are ordered by slot number.
      *  @note       In the Gasper paper, there is a definition of a epoch boundary pair (A, j).
@@ -149,7 +227,7 @@ module ForkChoiceHelpers {
         ensures |computeEBBs(xb, e)| == e as nat + 1
         /** The index for each epoch is in the range of xb. */
         ensures forall i :: 0 <= i < e as nat + 1 ==> computeEBBs(xb, e)[i] < |xb|
-        /** The sequence returned is in decreasing order. */
+        /** The sequence returned is in decreasing order slot-wise. */
         ensures forall i :: 1 <= i < e as nat + 1 ==> 
             xb[computeEBBs(xb, e)[i - 1]].slot >= xb[computeEBBs(xb, e)[i]].slot
         /** The epoch e - i boundary block has a slot less than (e - i) * SLOTS_PER_EPOCH. */
@@ -174,6 +252,42 @@ module ForkChoiceHelpers {
         )
     }
 
+    function computeEBBsFromRoots(xb : seq<Root>, e :  Epoch, store: Store) : seq<nat>
+        requires |xb| >= 1
+        requires forall r :: r in xb ==> r in store.blocks.Keys 
+        /** Last block has slot 0. */
+        requires store.blocks[xb[|xb| - 1]].slot == 0 
+
+        /** Each epoch has a block associated to. */
+        ensures |computeEBBsFromRoots(xb, e, store)| == e as nat + 1
+        /** The index for each epoch is in the range of xb. */
+        ensures forall i :: 0 <= i < e as nat + 1 ==> computeEBBsFromRoots(xb, e, store)[i] < |xb|
+        /** The sequence returned is in decreasing order slot-wise. */
+        ensures forall i :: 1 <= i < e as nat + 1 ==> 
+            store.blocks[xb[computeEBBsFromRoots(xb, e, store)[i - 1]]].slot >= store.blocks[xb[computeEBBsFromRoots(xb, e, store)[i]]].slot
+        /** The epoch e - i boundary block has a slot less than (e - i) * SLOTS_PER_EPOCH. */
+        ensures forall i :: 0 <= i < e as nat + 1 
+            ==> store.blocks[xb[computeEBBsFromRoots(xb, e, store)[i]]].slot as nat <= (e as nat - i) * SLOTS_PER_EPOCH as nat 
+        /** The  blocks at index j less than the epoch e - i boundary block have a slot 
+            larger than  (e - i) * SLOTS_PER_EPOCH. */
+        ensures forall i :: 0 <= i < e as nat + 1 ==> 
+            forall j :: 0 <= j < computeEBBsFromRoots(xb, e, store)[i] ==>
+            store.blocks[xb[j]].slot as nat > (e as nat - i) * SLOTS_PER_EPOCH as nat
+
+        decreases e 
+    {
+        //  Get the first boundary block
+        [computeFirstEBBIndexFromRoots(xb, e, store)] +
+        (
+            //  if e > 0 recursive call, otherwise, terminate.
+            if e == 0 then 
+                []
+            else 
+                computeEBBsFromRoots(xb, e - 1, store)
+        )
+    }
+
+
     /**
      *  LEBB definition.
      *
@@ -188,7 +302,7 @@ module ForkChoiceHelpers {
             && store.blocks[store.blocks[k].parent_root].slot < store.blocks[k].slot
         
     {
-        //  seq if beacon blocks (ancestors of br)
+        //  seq of beacon blocks (ancestors of br)
         var ch := chain(br, store);
         var bl := store.blocks[br];
         var slot := bl.slot;
@@ -196,23 +310,94 @@ module ForkChoiceHelpers {
         ch[lebbIndex]
     }
 
+    /**
+     *  Justified pairs in a view.
+     *  @param  xb  A view.
+     *  @param  xe  A sequence of indices such (xb[xe[j]], j) is a EBB at epoch j in `xb`.
+     *  @param  
+     *  @returns    The subset of indices in `xe` that are justified.
+     *  @note       xe[|xe| - 1] must be the last block in `xb` and this last block'slot is zero.
+     *              
+     */
+    // function justifiedPairs(xb : seq<BeaconBlock>, xe: seq<nat>, links : set<PendingAttestation>) : seq<nat>
+    //     requires |xb| >= 1
+    //     requires |xe| >= 1
+    //     /** Last block has slot 0. */
+    //     requires xb[|xb| - 1].slot == 0 
+    //     /** Indices in xe points to blocks in xe. */
+    //     requires forall i :: 0 <= i < |xe| ==> xe[i] < |xb|
+    //     /** Values in xe are decreasing. */
+    //     requires forall i :: 1 <= i < |xe| ==> xe[i - 1] <= xe[i]
+    //     /** Te last value is last block in `xb`. */
+    //     requires xe[|xe| - 1] == |xb| - 1
+    // {
+    //     //  last index is justified as it is the genesis block
+    //     if |xe| == 1 then 
+    //         [0]
+    //     else 
+    //         //
+    //         []
+    // }
 
     /**
      *  Justification definition.
      *  
-     *  @param  c   A checkpoint.
-     *  @param   
+     *  @param  i           An index in `xv`.
+     *  @param  xv          A sequence of EBB ordered by epochs from largest (first) to 0 (last).
+     *                      Each (xv.0, xv.1) is an EBB for epoch xv.1.
+     *  @param  links       The attestations with src and tgt checkpoints.
+     *  @param  refSet      A non-negative int typically the number of validators.
+     *  @returns            Whether the pair (b, i) in `xv` is justified.
+     *
+     *  @note               The difficulty (if any) here is that `xv` has blocks but
+     *                      links has attestations wich src and target that are roots.
+     *                      So we need the store and the map root --> block to make the link.   
      */
-    // predicate isJustified(c: CheckPoint, store: Store, genesisBlockRoot: Root ) 
+    predicate isJustified(i: nat, xv : seq<CheckPoint>, links : seq<PendingAttestation>, refSet: nat) 
+        requires |xv| >= 1
+        requires i < |xv|
+        /** SuperMajority link requires src.epoch < tgt.epoch. */
+        // requires forall i, j :: 0 <= i < j < |xv| ==> xv[i].epoch > xv[j].epoch
+        decreases |xv| - i 
+    {
+        if i == |xv| - 1 then 
+            //  Genesis block with slot 0 is justified.
+            true
+        else 
+            //  there should be a justified block at a higher index
+            exists j {:induction j} :: i < j < |xv| - 1 && isJustified(j, xv, links, refSet) 
+                && superMajorityLink(xv[j], xv[i], links, refSet)
+    }
+
+    /**
+     *  Whether links has an attestation from c1 to c2.
+     */
+    // predicate link(c1: (BeaconBlock, nat), c2: (BeaconBlock, nat), links : set<PendingAttestation>, store: Store)
+    //     /** Attestations must be for blocks in the store. */
+    //     requires forall a :: a in links ==>
+    //         a.data.source.root in store.blocks && a.data.target.root in store.blocks 
     // {
-    //     if c.epoch == 0 then 
-    //         // should be genesis block
-    //         c.root ==  genesisBlockRoot
-    //     else 
-    //         exists b1 :: b1 in strictChain(c.root, store) && isJustified(b1, store, genesisBlockRoot)
-    //         // && superMajority()
+    //     exists a :: a in links 
+    //         && c1 == (store.blocks[a.data.source.root], a.data.source.epoch as nat)  
     // }
 
-    
+    /**
+     *  
+     */
+    // function method countAttestationsForLinkBlocks(xa : seq<PendingAttestation>, linksrc : (BeaconBlock, nat), linktgt: (BeaconBlock, nat)) : nat
+    //     ensures countAttestationsForLinkBlocks(xa, linksrc, linktgt) <= |xa|
+    //     decreases xa
+    // {
+    //     // countAttestationsForLink()
+    //     0
+    //     // if |xl| == 0 then 
+    //     //     0
+    //     // else 
+    //     //     (if xl[0].data.source.root == linksrc && xl[0].data.target.root == linktgt then 
+    //     //         1
+    //     //     else 
+    //     //         0
+    //     //     ) + countAttestationsForLink(xl[1..], linksrc, linktgt)
+    // }
 
 }
